🧩 풀이 과정

<p><strong>[단계 1]</strong> 전체확률 $1$와 기댓값을 \(a,b,k\)로 표현한다.</p> <div class="math-display">$$ a+\sum_{x=1}^{k}\frac{b}{x}=1\$$</div> <div class="math-display">$$ E(X)=\sum_{x=1}^{k}x\cdot \frac{b}{x}=kb,\qquad E(X^2)=\sum_{x=1}^{k}x^2\cdot \frac{b}{x}=b\sum_{x=1}^{k}x=b\frac{k(k+1)}{2}. $$</div> <p><strong>[단계 2]</strong> 조건 \(E(X^2)=2E(X)\)을 이용해 \(k\)를 결정한다.</p> <div class="math-display">$$ b\frac{k(k+1)}{2}=2\cdot (kb)\ \Rightarrow\ \frac{k(k+1)}{2}=2k \ \Rightarrow\ k+1=4\ \Rightarrow\ k=3. $$</div> <p><strong>[단계 3]</strong> \(k=3\)일 때 \(a\)와 분산을 \(b\)로 나타낸다.</p> <div class="math-display">$$ 1+\frac12+\frac13=\frac{11}{6},\qquad a=1-\frac{11}{6}b. $$</div> <div class="math-display">$$ V(X)=E(X^2)-[E(X)]^2=2E(X)-[E(X)]^2=2(3b)-(3b)^2=6b-9b^2. $$</div> <p><strong>[단계 4]</strong> \(V(X)\)의 최대값을 주는 \(b\)를 구하고, 대응하는 \(a\)를 구한다.</p> <div class="math-display">$$ V(b)=6b-9b^2=-9(x-\frac13)^2+1 \Rightarrow\ b=\frac13\text{에서 최대} $$</div> <div class="math-display">$$ a=1-\frac{11}{6}\cdot\frac13=1-\frac{11}{18}=\frac{7}{18}. $$</div>

✅ 정답: $25$