🧩 풀이 과정

<p><strong>[단계 1]</strong> 확률의 합이 1이라는 조건을 이용한다.</p> <div class="math-display">$$ a + (a + b) + b = 1 $$</div> <div class="math-display">$$ 2a + 2b = 1 \Rightarrow a + b = \frac{1}{2} $$</div> <p><strong>[단계 2]</strong>\( E(X^2) \)를 식으로 나타낸다.</p> <div class="math-display">$$ E(X^2) = 1^2 a + 2^2 (a + b) + 3^2 b = a + 4(a + b) + 9b = 5a + 13b$$</div><p><strong>[단계 3]</strong> 문제에서 \( E(X^2) = a + 5 \)이므로 다음을 얻는다.</p> <div class="math-display">$$ 5a + 13b = a + 5 $$</div> <div class="math-display">$$ 4a + 13b = 5 $$</div> <p><strong>[단계 4]</strong> 연립방정식</p> <div class="math-display"> \[ \begin{cases} a + b = \frac{1}{2} \\ 4a + 13b = 5 \end{cases} \] </div> <p>이를 풀면,</p> <div class="math-display">$$ a = \frac{1}{6}, \quad b = \frac{1}{3} $$</div> <p><strong>[단계 5]</strong> 구하는 값은 \( b - a \)이다.</p> <div class="math-display">$$ b - a = \frac{1}{3} - \frac{1}{6} = \frac{1}{6} $$</div>

✅ 정답: ② $\frac{1}{6}$