🧩 풀이 과정

<p><strong>[단계 1]</strong> 주어진 조건 \(P(X=k)=P(X=k+2)\,(k=0,1,2)\)에서 확률들을 묶는다.</p> <p>\(X\)는 \(0,1,2,3,4\)를 가지므로 \(P(0)=P(2)=P(4)=p\), \(P(1)=P(3)=q\)라 두면, 전체 확률의 합은</p> <div class="math-display">$$3p+2q=1 \quad\Rightarrow\quad q=\frac{1-3p}{2}.$$</div> <p><strong>[단계 2]</strong> \(E(X^2)\)를 계산한다.</p> <div class="math-display">$$ E(X^2)=0^2P(0)+1^2P(1)+2^2P(2)+3^2P(3)+4^2P(4) =20p+10q. $$</div> <p>문제에서 \(E(X^2)=\dfrac{35}{6}\) 이므로</p> <div class="math-display">$$20p+10q=\frac{35}{6}\;\;\Longleftrightarrow\;\;4p+2q=\frac{7}{6}.$$</div> <p><strong>[단계 3]</strong> 연립하여 \(p\)를 구한다.</p> <div class="math-display">$$ \begin{cases} 3p+2q=1\\ 4p+2q=\dfrac{7}{6} \end{cases} \;\Rightarrow\; p=\frac{1}{6},\quad q=\frac{1}{4}. $$</div> <p><strong>[단계 4]</strong> 구하는 값은 \(P(X=0)=p\) 이다.</p> <div class="math-display">$$ P(X=0)=\frac{1}{6} $$</div>

✅ 정답: ④ $\frac{1}{6}$

<table> <thead> <tr><th>\(x\)</th><th>0</th><th>1</th><th>2</th><th>3</th><th>4</th><th>합</th></tr> </thead> <tbody> <tr><td>\(P(X=x)\)</td><td>\(p\)</td><td>\(q\)</td><td>\(p\)</td><td>\(q\)</td><td>\(p\)</td><td>\(1\)</td></tr> <tr><td>\(x^2P(X=x)\)</td><td>\(0\)</td><td>\(q\)</td><td>\(4p\)</td><td>\(9q\)</td><td>\(16p\)</td><td>\(E(X^2)\)</td></tr> </tbody> </table>